spot/GC.SPOT.ConcreteCallFull.fsti
@@ -49,57 +49,14 @@ let spot_gen_gc_success_post
 fn call_concrete_gen_gc_spot
   (r: unit{ConcreteMajor.spot_major_room})
   (gh: gen_heap_t)
-  (roots: array U64.t) (nroots: SZ.t)
-  (fwd_arr: array U64.t)
-  (queue: larray U64.t CheneyImpl.queue_size)
-  (slots: array U64.t) (nslots: SZ.t)
-  (st: gray_stack)
   requires is_gen_heap gh ConcreteMinor.spot_minor2.data ConcreteMinor.spot_minor2.bump
-             (ConcreteMajor.spot_major_heap r) (ConcreteMajor.spot_major_fp r) **
-           pts_to roots (ThreeObjects.spot_roots (ConcreteMajor.spot_c r)) **
-           pts_to fwd_arr ConcreteScenarios.spot_fwd_array **
-           pts_to queue 'qv **
-           pts_to slots (ThreeObjects.spot_slots (ConcreteMajor.spot_c r)) **
-           is_gray_stack st Seq.empty **
-           pure (
-             SZ.v nroots == 2 /\
-             SZ.v nslots == 1 /\
-             stack_capacity st >= 2)
+            (ConcreteMajor.spot_major_heap r) (ConcreteMajor.spot_major_fp r)
   returns res: (U64.t & bool)
-  ensures exists* d2 b2 final_major roots_out farr_out qv_out st_out.
+  ensures exists* d2 b2 final_major.
     is_gen_heap gh d2 b2 final_major (fst res) **
-    pts_to roots roots_out **
-    pts_to fwd_arr farr_out **
-    pts_to queue qv_out **
-    pts_to slots (ThreeObjects.spot_slots (ConcreteMajor.spot_c r)) **
-    is_gray_stack st st_out **
     pure (
-      let result =
-        CheneySpec.cheney_collect_spec
-          ConcreteMinor.spot_minor2
-          (ConcreteMajor.spot_major_heap r)
-          (ConcreteMajor.spot_major_fp r)
-          (ThreeObjects.spot_roots (ConcreteMajor.spot_c r)) in
       let ok = snd res in
-      GenImpl.gen_gc_roots_post
-        ConcreteMinor.spot_minor2
-        (ConcreteMajor.spot_major_heap r)
-        (ConcreteMajor.spot_major_fp r)
-        (ThreeObjects.spot_roots (ConcreteMajor.spot_c r))
-        roots_out Seq.empty (stack_capacity st) /\
       GenImpl.gen_gc_heap_shape_post d2 b2 final_major /\
-      GenImpl.gen_gc_reachable_subgraph_isomorphism_post
-        ConcreteMinor.spot_minor2
-        (ConcreteMajor.spot_major_heap r)
-        (ConcreteMajor.spot_major_fp r)
-        (ThreeObjects.spot_roots (ConcreteMajor.spot_c r))
-        ok final_major roots_out Seq.empty (stack_capacity st) /\
-      GenImpl.gen_gc_unreachable_final_blue_post
-        ConcreteMinor.spot_minor2
-        (ConcreteMajor.spot_major_heap r)
-        (ConcreteMajor.spot_major_fp r)
-        (ThreeObjects.spot_roots (ConcreteMajor.spot_c r))
-        final_major Seq.empty (stack_capacity st) /\
       Postconditions.minor_not_promoted
         ConcreteMinor.spot_minor2
         (ConcreteMajor.spot_major_heap r)
