spot/GC.SPOT.ConcreteSetup.fsti
@@ -1,0 +1,26 @@
+module GC.SPOT.ConcreteSetup
+
+module U64 = FStar.UInt64
+module Seq = FStar.Seq
+
+open GC.Spec.Base
+
+module CheneyImpl = GC.Gen.Impl.Cheney
+module Layout = GC.SPOT.Layout
+module ConcreteScenarios = GC.SPOT.ConcreteScenarios
+module ThreeObjects = GC.SPOT.ThreeObjects
+
+val spot_roots_alloc_seq
+  : c:obj_addr ->
+    Lemma (Seq.upd (Seq.create 2 (c <: U64.t)) 1 Layout.a_minor ==
+           ThreeObjects.spot_roots c)
+
+val spot_slots_alloc_seq
+  : c:obj_addr{U64.v c + Layout.c_to_a_field_index * 8 + 8 <= heap_size} ->
+    Lemma (Seq.create 1 ((ThreeObjects.spot_c_to_a_slot c) <: U64.t) ==
+           ThreeObjects.spot_slots c)
+
+val spot_fwd_alloc_seq
+  : unit ->
+    Lemma (Seq.create (FStar.SizeT.v CheneyImpl.queue_size_sz) 0UL ==
+           ConcreteScenarios.spot_fwd_array)
